One.one -> 1 except where it's hard

Iris/Iris/Instances/Lib/CInvariants.lean
@@ -45,7 +45,7 @@ def excl (γ : GName) : IProp GF := iOwn (E := W.inv) γ (some (Excl.excl ()), n
 
 @[rocq_alias cinv]
 def cinv (N : Namespace) (γ : GName) (P : IProp GF) : IProp GF :=
-  inv N iprop(P ∗ excl γ ∨ own γ (One.one : Qp))
+  inv N iprop(P ∗ excl γ ∨ own γ (1 : Qp))
 
 /-! ## Instances -/
 
@@ -102,9 +102,9 @@ instance instAsFractionalOwn (γ : GName) (q : Qp) :
 
 @[rocq_alias cinv_own_excl_alloc]
 theorem own_excl_alloc (P : GName → Prop) (HP : PredInfinite P) :
-    ⊢@{IProp GF} |==> ∃ γ, ⌜P γ⌝ ∗ excl γ ∗ own γ (One.one : Qp) := by
+    ⊢@{IProp GF} |==> ∃ γ, ⌜P γ⌝ ∗ excl γ ∗ own γ (1 : Qp) := by
   imod iOwn_alloc_strong (E := W.inv)
-    ((some (Excl.excl ()), none) • (none, some (One.one : Qp)) :
+    ((some (Excl.excl ()), none) • (none, some (1 : Qp)) :
       CInvF (IProp GF) (IProp GF)) P ?_
     ⟨trivial, Qp.valid_one⟩ with ⟨%γ, %HPγ, Hown⟩
   · intro N
@@ -120,10 +120,10 @@ theorem own_excl_alloc (P : GName → Prop) (HP : PredInfinite P) :
 
 @[rocq_alias cinv_own_1_l]
 theorem own_one_l {γ : GName} {q : Qp} :
-    ⊢ own (GF := GF) γ (One.one : Qp) -∗ own γ q -∗ False := by
+    ⊢ own (GF := GF) γ (1 : Qp) -∗ own γ q -∗ False := by
   iintro H1 H2
   icases own_valid $$ H1 H2 with %H
-  exact absurd H (by have := q.2; have : (One.one : Qp).val = 1 := rfl; grind)
+  exact absurd H (by have := q.2; have : (1 : Qp).val = 1 := rfl; grind)
 
 @[rocq_alias cinv_excl_excl]
 theorem excl_excl (γ : GName) :
@@ -156,7 +156,7 @@ nonrec theorem cinv_iff {N : Namespace} {γ : GName} {P Q : IProp GF} :
 
 @[rocq_alias cinv_alloc_strong]
 theorem alloc_strong (P : GName → Prop) (HP : PredInfinite P) (E : CoPset) (N : Namespace) :
-    ⊢@{IProp GF} |={E}=> ∃ γ, ⌜P γ⌝ ∗ own γ (One.one : Qp) ∗
+    ⊢@{IProp GF} |={E}=> ∃ γ, ⌜P γ⌝ ∗ own γ (1 : Qp) ∗
       ∀ Q, ▷ Q ={E}=∗ cinv N γ Q := by
   imod own_excl_alloc P HP with ⟨%γ, %HPγ, Hexcl, Hown⟩
   imodintro
@@ -172,7 +172,7 @@ theorem alloc_strong (P : GName → Prop) (HP : PredInfinite P) (E : CoPset) (N 
 @[rocq_alias cinv_alloc_strong_open]
 theorem alloc_strong_open (P : GName → Prop) (HP : PredInfinite P) (E : CoPset) (N : Namespace)
   (Hsub : ↑N ⊆ E) :
-    ⊢@{IProp GF} |={E}=> ∃ γ, ⌜P γ⌝ ∗ own γ (One.one : Qp) ∗
+    ⊢@{IProp GF} |={E}=> ∃ γ, ⌜P γ⌝ ∗ own γ (1 : Qp) ∗
       ∀ (Q : IProp GF), |={E, E \ ↑N}=> cinv N γ Q ∗ (▷ Q ={E \ ↑N, E}=∗ True) := by
   imod own_excl_alloc P HP with ⟨%γ, %HPγ, Hexcl, Hown⟩
   imodintro
@@ -180,7 +180,7 @@ theorem alloc_strong_open (P : GName → Prop) (HP : PredInfinite P) (E : CoPset
   iframe %HPγ Hown
   iframe
   iintro %Q
-  imod inv_alloc_open N E iprop(Q ∗ excl γ ∨ own γ (One.one : Qp)) Hsub with ⟨HI, Hclose⟩
+  imod inv_alloc_open N E iprop(Q ∗ excl γ ∨ own γ (1 : Qp)) Hsub with ⟨HI, Hclose⟩
   imodintro
   unfold cinv
   iframe
@@ -192,13 +192,13 @@ theorem alloc_strong_open (P : GName → Prop) (HP : PredInfinite P) (E : CoPset
 
 @[rocq_alias cinv_alloc_cofinite]
 theorem alloc_cofinite (G : List GName) (E : CoPset) (N : Namespace) :
-    ⊢@{IProp GF} |={E}=> ∃ γ, ⌜γ ∉ G⌝ ∗ own γ (One.one : Qp) ∗
+    ⊢@{IProp GF} |={E}=> ∃ γ, ⌜γ ∉ G⌝ ∗ own γ (1 : Qp) ∗
       ∀ Q, ▷ Q ={E}=∗ cinv N γ Q :=
   alloc_strong (· ∉ G) (PredInfinite.not_mem G) E N
 
 @[rocq_alias cinv_alloc]
 theorem alloc (E : CoPset) (N : Namespace) (P : IProp GF) :
-    ⊢ ▷ P ={E}=∗ ∃ γ, cinv N γ P ∗ own γ (One.one : Qp) := by
+    ⊢ ▷ P ={E}=∗ ∃ γ, cinv N γ P ∗ own γ (1 : Qp) := by
   iintro HP
   imod alloc_cofinite [] E N with ⟨%γ, %Hγ, Hown, Halloc⟩
   imod Halloc $$ HP with HI
@@ -208,7 +208,7 @@ theorem alloc (E : CoPset) (N : Namespace) (P : IProp GF) :
 
 @[rocq_alias cinv_alloc_open]
 theorem alloc_open (E : CoPset) (N : Namespace) (P : IProp GF) (Hsub : ↑N ⊆ E) :
-    ⊢@{IProp GF} |={E, E \ ↑N}=> ∃ γ, cinv N γ P ∗ own γ (One.one : Qp) ∗
+    ⊢@{IProp GF} |={E, E \ ↑N}=> ∃ γ, cinv N γ P ∗ own γ (1 : Qp) ∗
       (▷ P ={E \ ↑N, E}=∗ True) := by
   imod alloc_strong_open (fun _ => True) PredInfinite.true E N Hsub
     with ⟨%γ, _, Hown, Hmake⟩
@@ -221,7 +221,7 @@ theorem alloc_open (E : CoPset) (N : Namespace) (P : IProp GF) (Hsub : ↑N ⊆ 
 theorem acc_strong (E : CoPset) (N : Namespace) (γ : GName) (p : Qp) (P : IProp GF)
     (Hsub : ↑N ⊆ E) :
     ⊢ cinv N γ P -∗ own γ p ={E, E \ ↑N}=∗
-      ▷ P ∗ own γ p ∗ ∀ (E' : CoPset), ▷ P ∨ own γ (One.one : Qp) ={E', ↑N ∪ E'}=∗ True := by
+      ▷ P ∗ own γ p ∗ ∀ (E' : CoPset), ▷ P ∨ own γ (1 : Qp) ={E', ↑N ∪ E'}=∗ True := by
   unfold cinv
   iintro #Hinv Hown
   imod inv_acc_strong _ _ _ Hsub $$ Hinv with ⟨(⟨HP, >Hexcl⟩ | >Hown'), Hclose⟩
@@ -252,8 +252,8 @@ theorem acc (E : CoPset) (N : Namespace) (γ : GName) (p : Qp) (P : IProp GF)
 
 @[rocq_alias cinv_acc_1]
 theorem acc_one (E : CoPset) (N : Namespace) (γ : GName) (P : IProp GF) (Hsub : ↑N ⊆ E) :
-    ⊢ cinv N γ P -∗ own γ (One.one : Qp) ={E}=∗
-      ▷ P ∗ (▷ P ={E}=∗ own γ (One.one : Qp)) := by
+    ⊢ cinv N γ P -∗ own γ (1 : Qp) ={E}=∗
+      ▷ P ∗ (▷ P ={E}=∗ own γ (1 : Qp)) := by
   iintro #Hinv Hγ
   unfold cinv
   imod inv_acc _ _ _ Hsub $$ Hinv with ⟨(⟨HP, >Hexcl⟩ | >Hγ'), Hclose⟩
@@ -274,7 +274,7 @@ theorem acc_one (E : CoPset) (N : Namespace) (γ : GName) (P : IProp GF) (Hsub :
 
 @[rocq_alias cinv_cancel]
 theorem cancel (E : CoPset) (N : Namespace) (γ : GName) (P : IProp GF) (Hsub : ↑N ⊆ E) :
-    ⊢ cinv N γ P -∗ own γ (One.one : Qp) ={E}=∗ ▷ P := by
+    ⊢ cinv N γ P -∗ own γ (1 : Qp) ={E}=∗ ▷ P := by
   iintro #Hinv Hγ
   imod acc_one _ _ _ _ Hsub $$ Hinv Hγ with ⟨HP, -⟩
   imodintro
