Iris/Iris/Algebra/Auth.lean
@@ -85,7 +85,7 @@ instance : UCMRA (Auth A) := View.instUCMRA
 @[rocq_alias auth_auth]
 abbrev auth (dq : DFrac) (a : A) : Auth A := View.Auth dq a
 
-abbrev authFull (a : A) : Auth A := Auth (DFrac.own One.one) a
+abbrev authFull (a : A) : Auth A := Auth (DFrac.own 1) a
 
 @[rocq_alias auth_frag]
 abbrev frag (b : A) : Auth A := Frag b
